

Exercice 1 Consider a n -sized sample (X_1, \dots, X_n) of iid r.v. such that $X_i \sim \mathcal{P}(\theta, \sigma^2)$, with $\theta > 0$ unknown.

We study the two estimators:

$$\hat{\theta}_n = \bar{X}_n, \quad \text{and} \quad \hat{\sigma}_n = \sqrt{\frac{1}{n-1} \sum_{i=1}^n (X_i - \bar{X}_n)^2}.$$

① - Are these estimators consistent?

• From the Strong Law of Large Numbers^(SLLN), since X_i are iid with

$$\mathbb{E}[X_i] = \theta < +\infty, \text{ we have } \bar{X}_n = \frac{1}{n} \sum_{i=1}^n X_i \xrightarrow[n \rightarrow +\infty]{\text{p.s.}} \mathbb{E}[X_i] = \theta$$

Hence $\hat{\theta}_n \xrightarrow[n \rightarrow +\infty]{\text{p.s.}} \theta \Rightarrow \hat{\theta}_n \xrightarrow[n \rightarrow +\infty]{\text{p}} \theta \Rightarrow \hat{\theta}_n$ is a consistent estimator of θ .

• $\hat{\sigma}_n$ is the square root of the second-order empirical moment:

$$\begin{aligned} \hat{\sigma}_n^2 &= \frac{1}{n-1} \sum_{i=1}^n (X_i - \bar{X}_n)^2 = \frac{1}{n-1} \left(\sum_{i=1}^n X_i^2 - 2\bar{X}_n \underbrace{\sum_{i=1}^n X_i}_{=n\bar{X}_n} + n\bar{X}_n^2 \right) \\ &= \frac{1}{n-1} \left[\sum_{i=1}^n X_i^2 - 2n\bar{X}_n^2 + n\bar{X}_n^2 \right] = \frac{1}{n-1} \sum_{i=1}^n X_i^2 - \frac{n}{n-1} (\bar{X}_n)^2 \end{aligned}$$

By the SLLN, we have: $\frac{1}{n} \sum_{i=1}^n X_i^2 \xrightarrow[n \rightarrow +\infty]{\text{p.s.}} \mathbb{E}[X_i^2] = \text{Var}(X_i) + (\mathbb{E}[X_i])^2 = 2\sigma^2$

$$\bar{X}_n \xrightarrow[n \rightarrow +\infty]{\text{p.s.}} \mathbb{E}[X_i] = \theta$$

Hence, $\hat{\sigma}_n \xrightarrow[n \rightarrow +\infty]{\text{p.s.}} \sqrt{2\sigma^2 - \sigma^2} = \sigma$ by continuity. $\hat{\sigma}_n$ is thus consistent.

② - Compute the Fisher information of X_i :

$$I_1(\theta) = - \mathbb{E} \left[\frac{d^2}{d\theta^2} \ln L(\theta; X) \right] \text{ with}$$

$$\ln L(\theta; x) = \ln f_X(x; \theta) = \ln \left(\frac{1}{\sqrt{2\pi\theta^2}} e^{-\frac{(x-\theta)^2}{2\theta^2}} \right)$$

$$= -\frac{1}{2} \ln(2\pi) - \frac{1}{2} \ln(\theta^2) - \frac{(x-\theta)^2}{2\theta^2} = l(\theta; x)$$

$$\rightarrow \frac{d}{d\theta} l(\theta; x) = -\frac{1}{2} \cancel{2\theta} \frac{1}{\theta^2} - \left(\frac{-2(x-\theta) \times 2\theta^2 - 4\theta(x-\theta)^2}{4\theta^4} \right)$$

$$= -\frac{1}{\theta} - \frac{1}{4\theta^4} (-4\theta^2 x + \cancel{4\theta^3} - 4\theta x^2 + 8\theta^2 x - \cancel{4\theta^3})$$

$$= -\frac{1}{\theta} - \frac{1}{4\theta^4} (4\theta^2 x - 4\theta x^2) = -\frac{1}{\theta} - \frac{x}{\theta^2} + \frac{x^2}{\theta^3}$$

$$\rightarrow \frac{d^2}{d\theta^2} l(\theta; x) = \frac{d}{d\theta} \left(-\frac{1}{\theta} - \frac{x}{\theta^2} + \frac{x^2}{\theta^3} \right) = +\frac{1}{\theta^2} - x \times -2\theta^{-3} + x^2 \times (-3)\theta^{-4}$$

$$= \frac{1}{\theta^2} + \frac{2x}{\theta^3} - \frac{3x^2}{\theta^4} = \text{Var}(X) + (\mathbb{E}(X))^2$$

$$\text{Thus } I_1(\theta) = - \mathbb{E} \left[\frac{1}{\theta^2} + \frac{2X}{\theta^3} - \frac{3X^2}{\theta^4} \right] = - \left[\frac{1}{\theta^2} + \frac{2}{\theta^3} \mathbb{E}(X) - \frac{3}{\theta^4} \mathbb{E}(X^2) \right]$$

$$= - \left[\frac{1}{\theta^2} + \frac{2}{\theta^3} \times \theta - \frac{3}{\theta^4} (\theta^2 + \theta^2) \right] = - \left(\frac{1}{\theta^2} + \frac{2}{\theta^2} - \frac{6}{\theta^2} \right) = \frac{3}{\theta^2}$$

③ - Is $\hat{\theta}_n$ an efficient estimator?

- $\hat{\theta}_n$ is unbiased, and $\text{Var}(\hat{\theta}_n) = \text{Var}(\bar{X}_n) = \frac{\text{Var}(X_i)}{n} = \frac{\theta^2}{n}$

- $\frac{1}{I_n(\theta)} = \frac{1}{n I_1(\theta)} = \frac{\theta^2}{3n} < \frac{\theta^2}{n} = \text{Var}(\hat{\theta}_n) \Rightarrow \hat{\theta}_n$ does not reach the Cramer-Rao bound \Rightarrow it is not efficient.

Exercise 2 Consider the sample (X_1, \dots, X_n) of iid random variables, where $X_i \sim \mathcal{N}(0, 1)$. (2)

① - $\forall i=1, \dots, n$, we know that $X_i^2 \sim \chi_1^2$, and that $\sum_{i=1}^n X_i^2 \sim \chi_n^2$. (Chi-square distribution with n degrees of freedom).

$$\begin{aligned} \textcircled{2} - \sum_{i=1}^n (X_i - \bar{X}_n)^2 &= \sum_{i=1}^n (X_i^2 - 2X_i\bar{X}_n + \bar{X}_n^2) = \sum_{i=1}^n X_i^2 - 2\bar{X}_n \sum_{i=1}^n X_i + n\bar{X}_n^2 \\ &= \sum_{i=1}^n X_i^2 - 2n\bar{X}_n^2 + n\bar{X}_n^2 = \sum_{i=1}^n X_i^2 - n\bar{X}_n^2. \end{aligned}$$

Now, consider the random vector $X = \begin{pmatrix} X_1 \\ \vdots \\ X_n \end{pmatrix}$ and $A \in \mathcal{M}_{n \times n}(\mathbb{R})$, such that $AA^t = A^tA = \mathbb{I}_n$, where the last column of A is $\begin{pmatrix} \frac{1}{\sqrt{n}} \\ \frac{1}{\sqrt{n}} \\ \vdots \\ \frac{1}{\sqrt{n}} \end{pmatrix}$.
Let $Z = A^t X$.

③ - What is the distribution of Z ?

$\forall i, X_i \sim \mathcal{N}(0, 1)$. $\left\{ \begin{array}{l} \Rightarrow X \text{ is a Gaussian vector, i.e. } X \sim \mathcal{N}_n(\mu, \Sigma) \\ \text{Moreover, } X_i \text{ are iid} \end{array} \right.$

where $\mu = \mathbb{E}[X] = \begin{pmatrix} \mathbb{E}[X_1] \\ \vdots \\ \mathbb{E}[X_n] \end{pmatrix} = \begin{pmatrix} 0 \\ \vdots \\ 0 \end{pmatrix}$ and $\Sigma = \text{Var}(X) = \begin{pmatrix} \text{Var}(X_1) & \dots & \text{Cov}(X_n, X_1) \\ \vdots & \ddots & \vdots \\ \text{Cov}(X_n, X_n) & \dots & \text{Var}(X_n) \end{pmatrix} = \mathbb{I}_n$

Finally, $X \sim \mathcal{N}_n\left(\begin{pmatrix} 0 \\ \vdots \\ 0 \end{pmatrix}, \begin{pmatrix} 1 & & 0 \\ & \ddots & \\ 0 & & 1 \end{pmatrix}\right)$.

④ - Remind that $Z = A^t X$. $\Rightarrow \bullet \mathbb{E}[Z] = \mathbb{E}[A^t X] = A^t \mathbb{E}[X] = A^t \underset{\substack{\text{column vector} \\ \text{of } 0}}{0_n} = 0_n$

$$\begin{aligned} \bullet \text{Var}(Z) &= \mathbb{E}[(Z - \mathbb{E}[Z])(Z - \mathbb{E}[Z])^t] = \mathbb{E}[(A^t X - \underbrace{\mathbb{E}[A^t X]}_{=0})(A^t X - \underbrace{\mathbb{E}[A^t X]}_{=0})^t] \\ &= \mathbb{E}[A^t X (A^t X)^t] = \mathbb{E}[A^t X X^t (A^t)^t] = \mathbb{E}[A^t X X^t A] = A^t \mathbb{E}[X X^t] A \end{aligned}$$

$$= A^t \mathbb{E}[(X - \underbrace{\mathbb{E}(X)}_{=0})(X - \underbrace{\mathbb{E}(X)}_{=0})^t] A = A^t \text{Var}(X) A = A^t I_n A = A^t A = I_n.$$

• $Z = A^t X$: each component Z_i of the random vector Z is a linear combination of independent random variables X_1, \dots, X_n , each $X_i \sim \mathcal{N}(0, 1)$.

Hence Z_i is Gaussian, and Z is also Gaussian: $Z \sim \mathcal{N}_n(0_n, I_n)$.

⑤ - We have

$$\sum_{i=1}^n Z_i^2 = Z^t Z = (A^t X)^t (A^t X) = X^t (A^t)^t (A^t X) = X^t A A^t X = X^t X = \sum_{i=1}^n X_i^2$$

$$\textcircled{6} - \begin{pmatrix} Z_1 \\ Z_2 \\ \vdots \\ Z_n \end{pmatrix} = A^t X = \begin{pmatrix} a_{11} & \dots & a_{1n-1} & \frac{1}{\sqrt{n}} \\ a_{21} & \dots & & \vdots \\ \vdots & & & \vdots \\ a_{n1} & \dots & & \frac{1}{\sqrt{n}} \end{pmatrix}^t \begin{pmatrix} X_1 \\ \vdots \\ X_n \end{pmatrix} = \begin{pmatrix} a_{11} & \dots & a_{n1} \\ \vdots & & \vdots \\ a_{1n-1} & \dots & \frac{1}{\sqrt{n}} \\ \frac{1}{\sqrt{n}} & \dots & \frac{1}{\sqrt{n}} \end{pmatrix} \begin{pmatrix} X_1 \\ \vdots \\ X_n \end{pmatrix}$$

$$\text{Therefore } Z_n = \frac{1}{\sqrt{n}} X_1 + \frac{1}{\sqrt{n}} X_2 + \dots + \frac{1}{\sqrt{n}} X_n = \frac{1}{\sqrt{n}} \sum_{i=1}^n X_i.$$

⑦ - We know that:

$$\begin{aligned} \rightarrow \sum_{i=1}^n (X_i - \bar{X}_n)^2 &= \sum_{i=1}^n X_i^2 - n(\bar{X}_n)^2 \stackrel{\textcircled{5} \text{ et } \textcircled{6}}{=} \sum_{i=1}^n Z_i^2 - \frac{n}{n^2} (\sum X_i)^2 = \sum_{i=1}^n Z_i^2 - \frac{(\sum X_i)^2}{n} \\ &= \sum_{i=1}^{n-1} Z_i^2 \\ \rightarrow \sum_{i=1}^n X_i^2 &\sim \chi_n^2, \quad \begin{matrix} Z_1 \sim \mathcal{N}(0, 1) \\ Z_i \text{ iid} \end{matrix} \end{aligned}$$

$$\text{Hence } Z_1^2 \sim \chi_1^2 \Rightarrow \sum_{i=1}^{n-1} Z_i^2 \sim \chi_{n-1}^2.$$

Exercise 3

Consider the continuous random variable X with density:

$$f_X(x) = c e^{-\theta x + 1} \mathbb{1}_{x \geq -1}, \text{ with } \theta > 0 \text{ unknown, } c \text{ a constant.}$$

① - We know that f_θ is a density: $\begin{cases} \text{it is continuous} \\ \text{it is positive} \\ \int_{\mathbb{R}} f_\theta = 1. \end{cases}$

(3)

$$\int_{\mathbb{R}} (c e^{-\theta x+1}) 1_{x \geq -1} dx = 1$$

$$\int_{-1}^{+\infty} c e^{-\theta x+1} dx = 1 \Leftrightarrow c e \left[-\frac{e^{-\theta x}}{\theta} \right]_{-1}^{+\infty} = 1$$

$$\text{Hence } c e \left(0 + \frac{e^\theta}{\theta} \right) = 1 \Leftrightarrow \frac{c}{\theta} e^{\theta+1} = 1 \Leftrightarrow c = \theta e^{-\theta-1}$$

$$\textcircled{2} - E[X] = \int_{\mathbb{R}} x f_\theta(x) dx = \int_{-\infty}^{+\infty} x \theta e^{-\theta-1} e^{-\theta x+1} 1_{x \geq -1} dx$$

$$= \int_{-1}^{+\infty} \theta x e^{-\theta(x+1)} dx = \theta \int_{-1}^{+\infty} \frac{x e^{-\theta(x+1)}}{u v'} dx = \theta \left[\left[\frac{x e^{-\theta(x+1)}}{\theta} \right]_{-1}^{+\infty} - \int_{-1}^{+\infty} \frac{e^{-\theta(x+1)}}{\theta} dx \right]$$

$$= \left[-x e^{-\theta(x+1)} \right]_{-1}^{+\infty} + \int_{-1}^{+\infty} e^{-\theta(x+1)} dx = (0 + (-1)e^0) + \left[-\frac{e^{-\theta(x+1)}}{\theta} \right]_{-1}^{+\infty} = -1 + \left(-0 + \frac{1}{\theta} \right)$$

Using the SLLN, we have: since $\begin{cases} X_i \text{ iid} \\ E[X_i] < \infty \end{cases} = \frac{1}{\theta} - 1$.

$$\bar{X}_n = \frac{1}{n} \sum_{i=1}^n X_i \xrightarrow[n \rightarrow +\infty]{a.s.} E[X_i] = \frac{1}{\theta} - 1 \text{ - The method of moments leads}$$

$$\text{To define the estimator } \hat{\theta}_n \text{ such that } \bar{X}_n = \frac{1}{\hat{\theta}_n} - 1 \Leftrightarrow \hat{\theta}_n = \frac{1}{1 + \bar{X}_n}$$

③ - let $g(x) = \frac{1}{1+x}$ - It is clear that $g(x)$ is a continuous function on $] -1, +\infty[$.

$$\text{Then by continuity, since } \bar{X}_n \xrightarrow[n \rightarrow +\infty]{a.s.} \frac{1}{\theta} - 1 \text{ then } g(\bar{X}_n) \xrightarrow[n \rightarrow +\infty]{a.s.} g\left(\frac{1}{\theta} - 1\right)$$

$$\text{i.e. } \hat{\theta}_n = g(\bar{X}_n) \xrightarrow[n \rightarrow +\infty]{a.s.} \frac{1}{1 + \frac{1}{\theta} - 1} = \theta \Rightarrow \hat{\theta}_n \text{ is thus strongly consistent.}$$

④ - We seek an exhaustive / complete / sufficient statistic for θ :
 Let us look at the likelihood function: $L(\theta; x)$.

$$L(\theta; x) = \int_{(x_1, \dots, x_n)} (x_1, \dots, x_n; \theta) \stackrel{X_i \text{ iid}}{=} \prod_{i=1}^n f_{\theta}(x_i) = \prod_{i=1}^n \theta e^{-1-\theta} e^{-\theta x_i + 1} \mathbb{1}_{x_i \geq 1}$$

$$\text{Hence } L(\theta; x) = \theta^n e^{-n\theta} e^{-\theta \sum_{i=1}^n x_i} \mathbb{1}_{\min(x_i) \geq 1} = (\theta e^{-\theta})^n e^{-\theta \sum_{i=1}^n x_i} \mathbb{1}_{\min(x_i) \geq 1}$$

By the factorization theorem of Fisher-Neyman:

t is a sufficient statistic \Leftrightarrow there exist 2 measurable functions f and g such that: $\forall x \in]-1; +\infty[$, $\forall \theta > 0$,

$$L(\theta; x) = g(t(x); \theta) h(x)$$

$$\text{Here } h(x) = \mathbb{1}_{\min(x_i) \geq -1}$$

$$g(t(x); \theta) = (\theta e^{-\theta})^n e^{-\theta \sum_{i=1}^n x_i}$$

We deduce that $T(X) = \sum_{i=1}^n X_i$ is a sufficient statistic.

⑤ - It is given that the density function of $T = \sum_{i=1}^n X_i$ is

$$f_T(t) = \frac{\theta^n (t+n)^{n-1}}{(n-1)!} e^{-\theta(t+n)} \mathbb{1}_{t \geq -n}$$

Denote $T_n = \hat{\theta}_n = (1 + \bar{X}_n)^{-1}$, what is the density h of $\hat{\theta}_n$?

$$\text{We have } T_n = \frac{1}{1 + \frac{1}{n} \sum_{i=1}^n X_i} = \frac{1}{1 + \frac{T}{n}}$$

$$F_{T_n}(t) = \mathbb{P}(T_n \leq t) = \mathbb{P}\left(\frac{1}{1 + \frac{T}{n}} \leq t\right) = \mathbb{P}\left(1 + \frac{T}{n} \geq \frac{1}{t}\right) = \mathbb{P}\left(\frac{T}{n} \geq \frac{1}{t} - 1\right)$$

$$= \mathbb{P}\left(T \geq \frac{n(1-t)}{t}\right) = 1 - \mathbb{P}\left(T \leq \frac{n(1-t)}{t}\right) = 1 - F_T\left(\frac{n(1-t)}{t}\right)$$

$$\Rightarrow f_{T_n}(t) = \frac{d}{dt} F_{T_n}(t) = \frac{d}{dt} \left(1 - F_T\left(\frac{n(1-t)}{t}\right)\right) = -\left(\frac{-nt - n(1-t)}{t^2}\right) f_T\left(\frac{n(1-t)}{t}\right)$$

Therefore $f_{T_n}(t) = \frac{n! + n - n!}{t^2} \frac{\theta^n \left(\frac{n(1-t)}{t} + n\right)^{n-1}}{(n-1)!} e^{-\theta \left(\frac{n(1-t)}{t} + n\right)} \mathbb{1}_{\frac{n(1-t)}{t} \geq -n}$ (4)

We get

$$f_{T_n}(t) = \frac{n}{t^2} \frac{\theta^n \left(\frac{n}{t}\right)^{n-1}}{(n-1)!} e^{-\theta \frac{n}{t}} \mathbb{1}_{\frac{1-t}{t} \geq -1}$$

$$= \frac{1}{t} \times \left(\frac{n}{t}\right) \left(\frac{n}{t}\right)^{n-1} \frac{\theta^n}{(n-1)!} e^{-\frac{n\theta}{t}} \mathbb{1}_{\frac{1}{t} \geq 0}$$

$$= \frac{1}{t} \left(\frac{\theta n}{t}\right)^n \frac{e^{-n\theta/t}}{(n-1)!} \mathbb{1}_{\frac{1}{t} \geq 0} = \mathbb{1}_{t \geq 0}$$

⑥ - We indeed have found the same density function:

$$h(z) = \frac{(n\theta)^n}{(n-1)!} z^{-n-1} e^{-n\theta/z} \mathbb{1}_{z \geq 0}$$

Let us compute $E[T_n]$: by definition,

$$E[T_n] = \int_{-\infty}^{+\infty} z h(z) dz = \int_{-\infty}^{+\infty} z \frac{(n\theta)^n}{(n-1)!} z^{-n-1} e^{-n\theta/z} \mathbb{1}_{z \geq 0} dz$$

$$= \int_0^{+\infty} \frac{(n\theta)^n}{(n-1)!} z^{-n} e^{-n\theta/z} dz \stackrel{z=1/t}{=} \int_0^{+\infty} \frac{(n\theta)^n}{(n-1)!} t^n e^{-n\theta t} \times -\frac{1}{t^2} dt$$

$$= + \int_0^{+\infty} \frac{(n\theta)^n}{(n-1)!} t^{n-2} e^{-n\theta t} dt = \frac{(n\theta)^n}{(n-1)!} \int_0^{+\infty} \underbrace{t^{n-2}}_u \underbrace{e^{-n\theta t}}_{v'} dt$$

$$= \frac{(n\theta)^n}{(n-1)!} \left[\left[-\frac{t^{n-2} e^{-n\theta t}}{n\theta} \right]_0^{+\infty} - \int_0^{+\infty} -\frac{e^{-n\theta t}}{n\theta} (n-2)t^{n-3} dt \right]$$

$$= \frac{(n\theta)^n}{(n-1)!} \left[(0-0) + \frac{n-2}{n\theta} \int_0^{+\infty} t^{n-3} e^{-n\theta t} dt \right]$$

almost the same integral as previously!

thus, iterating the same integration by parts leads to:

$$\begin{aligned} E[T_n] &= \frac{(n\theta)^n}{(n-1)!} \frac{(n-2)!}{(n\theta)^{n-2}} \int_0^{\infty} e^{-n\theta t} dt = \frac{(n\theta)^n}{(n-1)!} \frac{(n-2)!}{(n\theta)^{n-2}} \underbrace{\left[-\frac{e^{-n\theta t}}{n\theta} \right]_0^{\infty}}_{= 1/n\theta} \\ &= \frac{(n\theta)^2}{(n-1)} \times \frac{1}{n\theta} = \frac{n\theta}{n-1} \end{aligned}$$

⑦ - If $T_n = \hat{\theta}_n$ were an estimator of θ , T_n would be biased since

$$E[T_n] = \frac{n}{n-1} \theta \neq \theta - \text{However, it is asymptotically unbiased,}$$

$$\text{since } \lim_{n \rightarrow \infty} \frac{n}{n-1} \theta = \theta$$

An unbiased estimator would be $T'_n = \frac{n-1}{n} T_n$.